Call macro for concurrency WIP (waiting for stpdd 1.7)

theories/examples/call.v
@@ -3,9 +3,9 @@ From iris.proofmode Require Import tactics.
 From cap_machine Require Import logrel macros_helpers macros rules proofmode.
 
 Section call.
-  Context {Σ:gFunctors} {memg:memG Σ} {regg:regG Σ}
-          {nainv: logrel_na_invs Σ}
-          `{MP: MachineParameters}.
+  Context {Σ:gFunctors} {CP:CoreParameters} {memg:memG Σ} {regg:@regG Σ CP}
+          `{LK: static_spinlock.lockG Σ, MP: MachineParameters}.
+
 
   (* Macro for a heap based calling convention *)
 
@@ -42,11 +42,12 @@ Section call.
             (let Hneq := fresh "Hneq" in destruct Hne as [Hneq Hne])); auto.
 
 
-  Lemma store_locals_spec_middle
+  Lemma store_locals_spec_middle (i : CoreN)
         (* cont *) φ
         (* list of locals *) r1 locals mlocals wsr
         (* PC *) a p b e a_first a_last
-        (* capability for locals *) p_l b_l e_l a_l :
+        (* capability for locals *) p_l b_l e_l a_l
+    EN:
     isCorrectPC_range p b e a_first a_last →
     contiguous_between a a_first a_last →
     finz.dist a_l e_l = strings.length locals →
@@ -56,17 +57,17 @@ Section call.
     length locals = length wsr ->
 
     (▷ store_locals a r1 locals
-   ∗ ▷ PC ↦ᵣ WCap p b e a_first
-   ∗ ▷ r1 ↦ᵣ WCap p_l b_l e_l a_l
-   ∗ ▷ ([∗ map] r↦w ∈ mlocals, r ↦ᵣ w)
+   ∗ ▷ (i,PC) ↦ᵣ WCap p b e a_first
+   ∗ ▷ (i,r1) ↦ᵣ WCap p_l b_l e_l a_l
+   ∗ ▷ ([∗ map] r↦w ∈ mlocals, (i,r) ↦ᵣ w)
    ∗ ▷ (∃ ws, [[a_l,e_l]]↦ₐ[[ws]])
-   ∗ ▷ (PC ↦ᵣ WCap p b e a_last
-           ∗ r1 ↦ᵣ WCap p_l b_l e_l e_l
-           ∗ ([∗ map] r↦w ∈ mlocals, r ↦ᵣ w)
+   ∗ ▷ ((i,PC) ↦ᵣ WCap p b e a_last
+           ∗ (i,r1) ↦ᵣ WCap p_l b_l e_l e_l
+           ∗ ([∗ map] r↦w ∈ mlocals, (i,r) ↦ᵣ w)
            ∗ [[a_l,e_l]]↦ₐ[[wsr]]
            ∗ store_locals a r1 locals
-           -∗ WP Seq (Instr Executable) {{ φ }})
-   ⊢ WP Seq (Instr Executable) {{ φ }})%I.
+           -∗ WP (i, Seq (Instr Executable)) @EN {{ φ }})
+   ⊢ WP (i, Seq (Instr Executable)) @EN {{ φ }})%I.
   Proof.
     iIntros (Hvpc Hcont Hsize Hnz Hwa Hwb Hperm Hlength) "(>Hprog & >HPC& >Hr_t1& >Hlocals& >Hbl& Hcont)".
     iInduction (locals) as [|r locals] "IH" forall (a_l mlocals wsr a a_first Hvpc Hcont Hnz Hsize Hwb Hperm Hlength).
@@ -141,7 +142,7 @@ Section call.
       + iPureIntro. eapply isCorrectPC_range_restrict;[eauto|].
         assert (a_first + 1 = Some f0)%a;[iContiguous_next Hcont 0|].
         assert (f0 + 1 = Some f)%a;[iContiguous_next Hcont 1|].
-        split;[revert H H0;clear|clear];solve_addr.
+        split;[revert H H0;clear|clear];try solve_addr.
       + iPureIntro.
         assert (a_first + 1 = Some f0)%a;[iContiguous_next Hcont 0|].
         assert (f0 + 1 = Some f)%a;[iContiguous_next Hcont 1|].
@@ -178,11 +179,12 @@ Section call.
   Qed.
 
 
-  Lemma store_locals_spec
+  Lemma store_locals_spec i
         (* cont *) φ
         (* list of locals *) r1 mlocals locals wsr
         (* PC *) a p b e a_first a_last
-        (* capability for locals *) p_l b_l e_l :
+        (* capability for locals *) p_l b_l e_l
+    EN :
     isCorrectPC_range p b e a_first a_last →
     contiguous_between a a_first a_last →
     finz.dist b_l e_l = strings.length locals →
@@ -192,18 +194,18 @@ Section call.
     length locals = length wsr ->
 
     (▷ store_locals a r1 locals
-   ∗ ▷ PC ↦ᵣ WCap p b e a_first
-   ∗ ▷ r1 ↦ᵣ WCap p_l b_l e_l b_l
-   ∗ ▷ ([∗ map] r↦w ∈ mlocals, r ↦ᵣ w)
+   ∗ ▷ (i,PC) ↦ᵣ WCap p b e a_first
+   ∗ ▷ (i,r1) ↦ᵣ WCap p_l b_l e_l b_l
+   ∗ ▷ ([∗ map] r↦w ∈ mlocals, (i, r) ↦ᵣ w)
    ∗ ▷ (∃ ws, [[b_l,e_l]]↦ₐ[[ws]])
-   ∗ ▷ (PC ↦ᵣ WCap p b e a_last
-           ∗ r1 ↦ᵣ WCap p_l b_l e_l e_l
-           ∗ ([∗ map] r↦w ∈ mlocals, r ↦ᵣ w)
+   ∗ ▷ ((i,PC) ↦ᵣ WCap p b e a_last
+           ∗ (i,r1) ↦ᵣ WCap p_l b_l e_l e_l
+           ∗ ([∗ map] r↦w ∈ mlocals, (i, r) ↦ᵣ w)
            ∗ [[b_l,e_l]]↦ₐ[[wsr]]
            ∗ store_locals a r1 locals
-           -∗ WP Seq (Instr Executable) {{ φ }})
+           -∗ WP (i, Seq (Instr Executable)) @EN {{ φ }})
 
-   ⊢ WP Seq (Instr Executable) {{ φ }})%I.
+   ⊢ WP (i, Seq (Instr Executable)) @EN {{ φ }})%I.
   Proof.
     iIntros (Hvpc Hcont Hsize Hnz Hwa Hperm Hlen) "(>Hprog & >HPC& >Hr_t1& >Hlocals& >Hbl& Hcont)".
     iApply (store_locals_spec_middle with "[$HPC $Hprog $Hr_t1 $Hlocals $Hbl $Hcont]");eauto.
@@ -260,11 +262,29 @@ Section call.
     simpl. auto.
   Qed.
 
-  Lemma call_spec
-        (* call *) r1 mlocals mparams wadv
-        (* remaining registers *) (rmap rmap' : gmap RegName Word)
+
+Definition registers_s_core (i:CoreN) (regs : gset RegName) : gset (CoreN * RegName)
+  := set_map (fun r => (i,r)) regs.
+
+(* Requires newer version of stdpp *)
+Program Definition registers_map_core `{A : Type} (i:CoreN) (regs : gmap RegName A)
+  : gmap (CoreN * RegName) A := _.
+Next Obligation. Admitted.
+(* := kmap (fun r => (i,r)) regs. *)
+
+Lemma big_sepM_register_map_core (i : CoreN) (l : gmap RegName Word) :
+  ([∗ map] k↦y ∈ (registers_map_core i l), k ↦ᵣ y)
+  ⊣⊢ ([∗ map] k↦y ∈ l, (i, k) ↦ᵣ y).
+Proof.
+  iSplit ; iIntros "H".
+Admitted.
+
+
+  Lemma call_spec (i : CoreN)
+        (* call *) (r1 : RegName) (mlocals mparams : gmap RegName Word) (wadv : Word)
+        (* remaining registers *) (rmap rmap' : gmap (CoreN*RegName) Word)
         (* pc *) a p b e a_first a_last
-        (* malloc *) f_m b_m e_m mallocN EN
+        (* malloc *) f_m b_m e_m mallocN EN γ
         (* linking *) b_link a_link e_link a_entry
         (* cont *) φ :
     isCorrectPC_range p b e a_first a_last →
@@ -273,65 +293,79 @@ Section call.
     (a_link + f_m)%a = Some a_entry →
     strings.length (map_to_list mlocals).*1 > 0 →
 
-    dom (gset RegName) rmap = all_registers_s ∖ {[ PC; r_t0; r1 ]} ∖ (dom (gset RegName) mparams) ∖ (dom (gset RegName) mlocals) →
-    dom (gset RegName) rmap' = all_registers_s ∖ {[ PC; r_t0; r1 ]} ∖ (dom (gset RegName) mparams) →
-    {[r_t1; r_t2; r_t3; r_t4; r_t5; r_t6]} ⊆ dom (gset RegName) rmap → (* we need to know that neither params nor locals use these gen pur registers *)
+    dom (gset (CoreN*RegName)) rmap = ((all_registers_s_core i)
+                                          ∖ registers_s_core i {[ PC; r_t0; r1 ]}
+                                          ∖ registers_s_core i (dom (gset RegName) mparams)
+                                          ∖ registers_s_core i (dom (gset RegName) mlocals)) →
+    dom (gset (CoreN*RegName)) rmap' = ((all_registers_s_core i)
+                                          ∖ registers_s_core i {[ PC; r_t0; r1 ]}
+                                          ∖ registers_s_core i (dom (gset RegName) mparams)) →
+    registers_s_core i {[r_t1; r_t2; r_t3; r_t4; r_t5; r_t6]} ⊆
+      dom (gset (CoreN*RegName)) rmap → (* we need to know that neither params nor locals use these gen pur registers *)
     ↑mallocN ⊆ EN →
 
     (▷ call a f_m r1 (map_to_list mlocals).*1 (map_to_list mparams).*1
-    ∗ ▷ PC ↦ᵣ WCap p b e a_first
-    ∗ na_inv logrel_nais mallocN (malloc_inv b_m e_m)
-    ∗ na_own logrel_nais EN
+    ∗ inv mallocN (malloc_inv b_m e_m γ)
+    ∗ ▷ (i,PC) ↦ᵣ WCap p b e a_first
     (* we need to assume that the malloc capability is in the linking table at offset 0 *)
     ∗ ▷ b ↦ₐ WCap RO b_link e_link a_link
     ∗ ▷ a_entry ↦ₐ WCap E b_m e_m b_m
     (* registers *)
     ∗ ▷ ([∗ map] r_i↦w_i ∈ rmap, r_i ↦ᵣ w_i)
-    ∗ ▷ ([∗ map] r_i↦w_i ∈ mparams, r_i ↦ᵣ w_i)
-    ∗ ▷ (∃ w, r_t0 ↦ᵣ w)
-    ∗ ▷ r1 ↦ᵣ wadv
-    ∗ ▷ ([∗ map] r_i↦w_i ∈ mlocals, r_i ↦ᵣ w_i)
+    ∗ ▷ ([∗ map] r_i↦w_i ∈ mparams, (i, r_i) ↦ᵣ w_i)
+    ∗ ▷ (∃ w, (i,r_t0) ↦ᵣ w)
+    ∗ ▷ (i,r1) ↦ᵣ wadv
+    ∗ ▷ ([∗ map] r_i↦w_i ∈ mlocals, (i, r_i) ↦ᵣ w_i)
     (* continuation *)
     ∗ ▷ ((∃ b_c e_c b_l e_l a_end, ⌜(a_end + 1)%a = Some a_last⌝
-            ∗ PC ↦ᵣ updatePcPerm wadv
+            ∗ (i,PC) ↦ᵣ updatePcPerm wadv
             ∗ ([∗ map] r_i↦_ ∈ rmap', r_i ↦ᵣ WInt 0%Z)
-            ∗ ([∗ map] r_i↦w_i ∈ mparams, r_i ↦ᵣ w_i)
+            ∗ ([∗ map] r_i↦w_i ∈ mparams, (i, r_i) ↦ᵣ w_i)
             ∗ b ↦ₐ WCap RO b_link e_link a_link
             ∗ a_entry ↦ₐ WCap E b_m e_m b_m
-            ∗ r1 ↦ᵣ wadv
-            ∗ r_t0 ↦ᵣ WCap E b_c e_c b_c
+            ∗ (i,r1) ↦ᵣ wadv
+            ∗ (i, r_t0) ↦ᵣ WCap E b_c e_c b_c
             ∗ [[b_c,e_c]]↦ₐ[[ [WInt hw_1;WInt hw_2;WInt hw_3;WInt hw_4;WInt hw_5;WCap RWX b_l e_l e_l;WCap p b e a_end] ]]
             ∗ [[b_l,e_l]]↦ₐ[[ (map_to_list mlocals).*2 ]]
             ∗ call a f_m r1 (map_to_list mlocals).*1 (map_to_list mparams).*1
-            ∗ na_own logrel_nais EN)
-            -∗ WP Seq (Instr Executable) {{ φ }})
-    ⊢ WP Seq (Instr Executable) {{ λ v, φ v ∨ ⌜v = FailedV⌝ }})%I.
+            -∗ WP (i, Seq (Instr Executable)) @EN {{ φ }}))
+    ⊢ WP (i, Seq (Instr Executable)) @EN {{ λ v, φ v ∨ ⌜v = (i, FailedV)⌝ }})%I.
   Proof.
     iIntros (Hvpc Hcont Hwb Hlink Hnz Hdom1 Hdom2 Hsub Hnainv)
-            "(>Hprog & >HPC & #Hnainv & Hown & >Hb & >Ha_entry & >Hgen & >Hparams & >Hr_t0 & >Hr1 & >Hlocals & Hcont)".
+            "(>Hprog & #Hinv & >HPC & >Hb & >Ha_entry & >Hgen & >Hparams & >Hr_t0 & >Hr1 & >Hlocals & Hcont)".
     (* prepare the registers *)
     iDestruct "Hr_t0" as (w) "Hr_t0".
     iAssert (⌜mparams ##ₘmlocals⌝)%I as %Hdisj1.
-    { rewrite map_disjoint_spec. iIntros (i x y Hx Hy).
-      iDestruct (big_sepM_delete _ _ i with "Hparams") as "[Hi1 Hparams]";[eauto|].
-      iDestruct (big_sepM_delete _ _ i with "Hlocals") as "[Hi2 Hlocals]";[eauto|].
+    { rewrite map_disjoint_spec. iIntros (j x y Hx Hy).
+      iDestruct (big_sepM_delete _ _ j with "Hparams") as "[Hi1 Hparams]";[eauto|].
+      iDestruct (big_sepM_delete _ _ j with "Hlocals") as "[Hi2 Hlocals]";[eauto|].
       iDestruct (regname_dupl_false with "Hi1 Hi2") as "Hfalse". done. }
-    iAssert (⌜mparams ##ₘrmap⌝)%I as %Hdisj2.
-    { rewrite map_disjoint_spec. iIntros (i x y Hx Hy).
-      iDestruct (big_sepM_delete _ _ i with "Hparams") as "[Hi1 Hparams]";[eauto|].
-      iDestruct (big_sepM_delete _ _ i with "Hgen") as "[Hi2 Hgen]";[eauto|].
-      iDestruct (regname_dupl_false with "Hi1 Hi2") as "Hfalse". done. }
-    iAssert (⌜mlocals ##ₘrmap⌝)%I as %Hdisj3.
-    { rewrite map_disjoint_spec. iIntros (i x y Hx Hy).
-      iDestruct (big_sepM_delete _ _ i with "Hgen") as "[Hi1 Hgen]";[eauto|].
-      iDestruct (big_sepM_delete _ _ i with "Hlocals") as "[Hi2 Hlocals]";[eauto|].
-      iDestruct (regname_dupl_false with "Hi1 Hi2") as "Hfalse". done. }
+    iAssert ([∗ map] k↦y ∈ (registers_map_core i mparams), k ↦ᵣ y)%I
+    with "[Hparams]" as "Hparams".
+    { rewrite /registers_map_core.
+      (* rewrite /kmap. *)
+      admit. }
+
+    iAssert (⌜ registers_map_core i mparams ##ₘrmap⌝)%I as %Hdisj2.
+    { rewrite map_disjoint_spec. iIntros (j x y Hx Hy).
+      iDestruct (big_sepM_delete _ _ j with "Hgen") as "[Hi2 Hgen]";[eauto|].
+      (* iDestruct (big_sepM_delete _ _ (snd j) with "[Hparams]") as "[Hi1 Hparams]". ;[eauto|]. *)
+      (* iDestruct (regname_dupl_false with "Hi1 Hi2") as "Hfalse". done. } *)
+      admit. }
+    iAssert (⌜registers_map_core i mlocals ##ₘrmap⌝)%I as %Hdisj3.
+    { admit. }
+    (* { rewrite map_disjoint_spec. iIntros (i x y Hx Hy). *)
+    (*   iDestruct (big_sepM_delete _ _ i with "Hgen") as "[Hi1 Hgen]";[eauto|]. *)
+    (*   iDestruct (big_sepM_delete _ _ i with "Hlocals") as "[Hi2 Hlocals]";[eauto|]. *)
+    (*   iDestruct (regname_dupl_false with "Hi1 Hi2") as "Hfalse". done. } *)
     iAssert (⌜PC ∉ dom (gset RegName) mparams ∧ r_t0 ∉ dom (gset RegName) mparams ∧ r1 ∉ dom (gset RegName) mparams⌝)%I as %Hdisj4.
-    { repeat iSplit; iIntros (Hcontr); apply elem_of_gmap_dom in Hcontr as [? Hi];
-        (iDestruct (big_sepM_delete with "Hparams") as "[Hi1 Hparams]";[by eauto|]).
-      by iDestruct (regname_dupl_false with "Hi1 HPC") as "Hfalse".
-      by iDestruct (regname_dupl_false with "Hi1 Hr_t0") as "Hfalse".
-      by iDestruct (regname_dupl_false with "Hi1 Hr1") as "Hfalse".
+    {
+      (* iSplit; iIntros (Hcontr); apply elem_of_gmap_dom in Hcontr as [? Hi]. *)
+      (*   (iDestruct (big_sepM_delete with "Hparams") as "[Hi1 Hparams]";[by eauto|]). *)
+      (* by iDestruct (regname_dupl_false with "Hi1 HPC") as "Hfalse". *)
+      (* by iDestruct (regname_dupl_false with "Hi1 Hr_t0") as "Hfalse". *)
+      (* by iDestruct (regname_dupl_false with "Hi1 Hr1") as "Hfalse". *)
+      admit.
     }
     iAssert (⌜PC ∉ dom (gset RegName) mlocals ∧ r_t0 ∉ dom (gset RegName) mlocals ∧ r1 ∉ dom (gset RegName) mlocals⌝)%I as %Hdisj5.
     { repeat iSplit; iIntros (Hcontr); apply elem_of_gmap_dom in Hcontr as [? Hi];
@@ -340,46 +374,70 @@ Section call.
       by iDestruct (regname_dupl_false with "Hi1 Hr_t0") as "Hfalse".
       by iDestruct (regname_dupl_false with "Hi1 Hr1") as "Hfalse".
     }
-    iAssert (⌜∀ r, r ∈ {[r_t1; r_t2; r_t3; r_t4; r_t5; r_t6]} → r ≠ r1⌝)%I as %Hneregs.
+    iAssert (⌜∀ r, (i,r) ∈ registers_s_core i {[r_t1; r_t2; r_t3; r_t4; r_t5; r_t6]} → (i,r) ≠ (i,r1)⌝)%I as %Hneregs.
     { iIntros (r Hin Hcontr). subst. apply Hsub in Hin.
       apply elem_of_gmap_dom in Hin as [x Hx].
       iDestruct (big_sepM_delete with "Hgen") as "[Hr Hgen]";[apply Hx|].
+      inversion Hcontr ; subst.
       by iDestruct (regname_dupl_false with "Hr Hr1") as "Hfalse".
     }
 
-    iDestruct (big_sepM_union with "[$Hlocals $Hparams]") as "Hlocalsparams";[auto|].
-    iDestruct (big_sepM_union with "[$Hgen $Hlocalsparams]") as "Hgenlocalsparams";[apply map_disjoint_union_r_2;auto|].
-    iAssert (⌜(rmap ∪ (mlocals ∪ mparams)) !! r1 = None⌝)%I as %Hnone.
-    { destruct ((rmap ∪ (mlocals ∪ mparams)) !! r1) eqn:Hsome;auto.
-      iDestruct (big_sepM_delete _ _ r1 with "Hgenlocalsparams") as "[Hi1 Hgen]";[eauto|].
-      iDestruct (regname_dupl_false with "Hi1 Hr1") as "Hfalse". done. }
-    iAssert (⌜(rmap ∪ (mlocals ∪ mparams)) !! r_t0 = None⌝)%I as %Hnone'.
-    { destruct ((rmap ∪ (mlocals ∪ mparams)) !! r_t0) eqn:Hsome;auto.
-      iDestruct (big_sepM_delete _ _ r_t0 with "Hgenlocalsparams") as "[Hi1 Hgen]";[eauto|].
-      iDestruct (regname_dupl_false with "Hi1 Hr_t0") as "Hfalse". done. }
+    (* iDestruct (big_sepM_union with "[$Hlocals $Hparams]") as "Hlocalsparams" *)
+    (* ;[auto|]. *)
+
+    iAssert ([∗ map] k↦y ∈ (registers_map_core i (mlocals ∪ mparams)), k ↦ᵣ y)%I
+    with "[Hlocals Hparams]" as "Hlocalsparams".
+    { admit. }
+
+    iDestruct (big_sepM_union with "[$Hgen $Hlocalsparams]") as "Hgenlocalsparams"
+    ; [admit|].
+    (* ;[apply map_disjoint_union_r_2;auto|]. *)
+    iAssert (⌜(rmap ∪ registers_map_core i (mlocals ∪ mparams)) !! (i, r1) = None⌝)%I
+      as %Hnone.
+    { admit. }
+    (* { destruct ((rmap ∪ (mlocals ∪ mparams)) !! r1) eqn:Hsome;auto. *)
+    (*   iDestruct (big_sepM_delete _ _ r1 with "Hgenlocalsparams") as "[Hi1 Hgen]";[eauto|]. *)
+    (*   iDestruct (regname_dupl_false with "Hi1 Hr1") as "Hfalse". done. } *)
+    iAssert (⌜(rmap ∪ registers_map_core i (mlocals ∪ mparams)) !! (i, r_t0) = None⌝)%I as %Hnone'.
+    { admit. }
+    (* { destruct ((rmap ∪ (mlocals ∪ mparams)) !! r_t0) eqn:Hsome;auto. *)
+    (*   iDestruct (big_sepM_delete _ _ r_t0 with "Hgenlocalsparams") as "[Hi1 Hgen]";[eauto|]. *)
+    (*   iDestruct (regname_dupl_false with "Hi1 Hr_t0") as "Hfalse". done. } *)
     iAssert (⌜r1 ≠ PC⌝)%I as %Hne1.
     { iIntros (->). iDestruct (regname_dupl_false with "HPC Hr1") as "Hfalse". done. }
     iAssert (⌜r1 ≠ r_t0⌝)%I as %Hne2.
     { iIntros (->). iDestruct (regname_dupl_false with "Hr_t0 Hr1") as "Hfalse". done. }
-    iDestruct (big_sepM_insert with "[$Hgenlocalsparams $Hr1]") as "Hgenlocalsparams";[auto|].
+    iDestruct (big_sepM_insert with "[$Hgenlocalsparams $Hr1]") as
+      "Hgenlocalsparams";[eauto|].
 
-    assert (dom (gset RegName) (<[r1:=wadv]> (rmap ∪ (mlocals ∪ mparams))) = all_registers_s ∖ {[PC; r_t0]}) as Hdomeq.
+    assert (dom (gset (CoreN*RegName))
+              (<[(i, r1):=wadv]> (rmap ∪ (registers_map_core i (mlocals ∪ mparams))))
+            = all_registers_s_core i ∖ {[(i, PC); (i, r_t0)]}) as Hdomeq.
     { rewrite dom_insert_L !dom_union_L. revert Hdom1 Hne1 Hne2 Hdisj1 Hdisj2 Hdisj3 Hdisj4 Hdisj5. clear. intros Hdom1 Hne1 Hne2 Hdisj1 Hdisj2 Hdisj3 Hdisj4 Hdisj5.
-      assert (all_registers_s ∖ {[PC; r_t0]} = {[r1]} ∪ all_registers_s ∖ {[PC; r_t0; r1]}) as ->.
+      assert (all_registers_s_core i ∖ {[(i, PC); (i, r_t0)]}
+              = {[(i, r1)]} ∪ all_registers_s_core i ∖
+                  {[(i, PC); (i, r_t0); (i, r1)]}) as ->.
       { rewrite - !difference_difference_L.
         rewrite -union_difference_L; auto.
-        apply subseteq_difference_r;[set_solver|].
-        apply subseteq_difference_r;[set_solver|].
-        apply all_registers_subseteq. }
-      assert (dom (gset RegName) rmap ∪ (dom (gset RegName) mlocals ∪ dom (gset RegName) mparams) =
-              dom (gset RegName) mparams ∪ (dom (gset RegName) mlocals ∪ dom (gset RegName) rmap)) as ->.
-      { rewrite (union_comm_L _ (dom _ mparams)). rewrite union_assoc_L. rewrite (union_comm_L _ (dom _ mparams)).
-        rewrite -union_assoc_L. rewrite (union_comm_L _ (dom _ mlocals)). auto. }
-      rewrite Hdom1. rewrite - !difference_difference_L - !union_difference_L; auto.
-      repeat (apply subseteq_difference_r;[set_solver|]). apply all_registers_subseteq.
-      repeat (apply subseteq_difference_r;[set_solver|]). apply all_registers_subseteq.
-      apply subseteq_difference_r;[apply map_disjoint_dom;auto|].
-      repeat (apply subseteq_difference_r;[set_solver|]). apply all_registers_subseteq.
+        rewrite /all_registers_s_core.
+        admit. }
+        (* apply subseteq_difference_r;[set_solver|]. *)
+        (* apply subseteq_difference_r;[set_solver|]. *)
+        (* apply all_registers_subseteq. } *)
+      (* assert (dom (gset (CoreN * RegName)) rmap *)
+      (*           ∪ (dom (gset (CoreN * RegName)) (registers_map_core i mlocals) *)
+      (*                ∪ dom (gset (CoreN * RegName)) (registers_map_core i mparams)) = *)
+      (*         dom (gset (CoreN * RegName)) (registers_map_core i mparams) *)
+      (*           ∪ (dom (gset (CoreN * RegName)) (registers_map_core i mlocals) *)
+      (*                ∪ dom (gset (CoreN * RegName)) rmap)) as ->. *)
+      (* { rewrite (union_comm_L _ (dom _ mparams)). rewrite union_assoc_L. rewrite (union_comm_L _ (dom _ mparams)). *)
+      (*   rewrite -union_assoc_L. rewrite (union_comm_L _ (dom _ mlocals)). auto. } *)
+      (* rewrite Hdom1. rewrite - !difference_difference_L - !union_difference_L; auto. *)
+      (* repeat (apply subseteq_difference_r;[set_solver|]). apply all_registers_subseteq. *)
+      (* repeat (apply subseteq_difference_r;[set_solver|]). apply all_registers_subseteq. *)
+      (* apply subseteq_difference_r;[apply map_disjoint_dom;auto|]. *)
+      (* repeat (apply subseteq_difference_r;[set_solver|]). apply all_registers_subseteq. *)
+      admit.
     }
 
     (* malloc f_m |locals| *)
@@ -387,33 +445,46 @@ Section call.
         (malloc_prog rest1 link1) "(Hmalloc_prog & Hprog & #Hcont1)";[apply Hcont|].
     iDestruct "Hcont1" as %(Hcont1 & Hcont2 & Heqapp1 & Hlink1).
     rewrite -/(malloc _ _ _).
-    iApply (wp_wand_l _ _ _ (λne v, ((φ v ∨ ⌜v = FailedV⌝) ∨ ⌜v = FailedV⌝)))%I. iSplitR.
+    iApply (wp_wand_l _ _ _ (λne v, ((φ v ∨ ⌜v = (i, FailedV)⌝) ∨ ⌜v = (i, FailedV)⌝)))%I. iSplitR.
     { iIntros (v) "[H|H] /=";auto. }
-    iApply (malloc_spec with "[- $HPC $Hnainv $Hown $Hb $Ha_entry $Hmalloc_prog $Hr_t0 $Hgenlocalsparams]");auto;[|apply Hcont1|..].
-    { eapply isCorrectPC_range_restrict;eauto. split;[clear;solve_addr|]. apply contiguous_between_bounds in Hcont2. auto. }
-    iNext. iIntros "(HPC & Hmalloc & Hb & Ha_entry & Hregion & Hr_t0 & Hna & Hgenlocalsparams)".
+    iApply (malloc_spec with "[- $HPC $Hinv $Hb $Ha_entry $Hmalloc_prog $Hr_t0 $Hgenlocalsparams]");auto;[|apply Hcont1|..].
+    { eapply isCorrectPC_range_restrict;eauto. split;[clear;solve_addr|]. apply
+        contiguous_between_bounds in Hcont2. auto. }
+    eauto.
+    iNext. iIntros "(HPC & Hmalloc & Hb & Ha_entry & Hregion & Hr_t0 & Hgenlocalsparams)".
     iDestruct "Hregion" as (b_l e_l Hlocals_size) "(Hr_t1 & Hbl)".
 
     (* in order to store the locals, we need to extract locals from the map *)
-    rewrite !delete_insert_ne;auto. 2: { apply Hneregs. constructor. }
+    rewrite delete_insert_ne. 2: { apply Hneregs. rewrite /registers_s_core. set_solver+. }
     rewrite delete_union. rewrite !insert_union_l.
-    rewrite (delete_notin (mlocals ∪ mparams));[|disjoint_from_rmap rmap].
+    rewrite (delete_notin (registers_map_core i (mlocals ∪ mparams)))
+              ;[| admit].
+    (* [|disjoint_from_rmap rmap]. *)
     iDestruct (big_sepM_union with "Hgenlocalsparams") as "[Hgen Hlocalsparams]".
     { repeat (apply map_disjoint_insert_l_2;[disjoint_from_rmap rmap|]).
-      apply map_disjoint_insert_l_2. apply lookup_union_None in Hnone as [? ?];auto.
-      apply map_disjoint_delete_l. apply map_disjoint_union_r_2;auto. }
-    iDestruct (big_sepM_union with "Hlocalsparams") as "[Hlocals Hparams]";auto.
-
+      admit. }
+      (* apply map_disjoint_insert_l_2. apply lookup_union_None in Hnone as [? ?];auto. *)
+      (* apply map_disjoint_delete_l. apply map_disjoint_union_r_2;auto. } *)
+    (* iDestruct (big_sepM_union with "Hlocalsparams") as "[Hlocals Hparams]";auto. *)
+    iAssert ( ([∗ map] k↦y ∈ registers_map_core i (mlocals), k ↦ᵣ y)
+              ∗ ([∗ map] k↦y ∈ registers_map_core i (mparams), k ↦ᵣ y))%I
+      with "[Hlocalsparams]"
+      as "[Hlocals Hparams]".
+    { admit. }
     (* store locals *)
     iDestruct (contiguous_between_program_split with "Hprog") as
         (storelocals_prog rest2 link2) "(Hstorelocals_prog & Hprog & #Hcont2)";[apply Hcont2|].
     iDestruct "Hcont2" as %(Hcont3 & Hcont4 & Heqapp2 & Hlink2).
-    iApply (store_locals_spec _ _ _ _ ((map_to_list mlocals).*2) with "[- $HPC $Hstorelocals_prog $Hr_t1 $Hlocals]");[|apply Hcont3|auto..].
+    iAssert ([∗ map] k↦y ∈ mlocals, (i,k) ↦ᵣ y)%I with "[Hlocals]" as
+      "Hlocals" ; [admit|].
+    iApply (store_locals_spec _ _ _ _ ((map_to_list mlocals).*1) with "[-$HPC $Hstorelocals_prog $Hr_t1 $Hlocals]");[|apply Hcont3|auto..].
     { eapply isCorrectPC_range_restrict;[apply Hvpc|].
       apply contiguous_between_bounds in Hcont1.
       apply contiguous_between_bounds in Hcont4. auto. }
-    { clear -Hlocals_size. rewrite /finz.dist. solve_addr. }
-    { rewrite zip_fst_snd. auto. }
+    { clear - Hlocals_size.
+      rewrite /finz.dist. solve_addr. }
+    { Unshelve. 2: exact (map_to_list mlocals).*2.
+      rewrite zip_fst_snd. auto. }
     { apply length_fst_snd. }
     iSplitL "Hbl";[eauto|].
     iNext. iIntros "(HPC & Hr_t1 & Hmlocals & Hbl & Hstorelocals_prog)".
@@ -428,10 +499,15 @@ Section call.
     apply contiguous_between_cons_inv_first in Hcont4 as Heq; subst f.
 
     (* get some general purpose registers *)
-    assert (is_Some (rmap !! r_t6)) as [w6 Hw6];[apply elem_of_gmap_dom;apply Hsub;repeat constructor|].
-    iDestruct (big_sepM_delete _ _ r_t6 with "Hgen") as "[Hr_t6 Hgen]".
-    { assert (r_t6 ≠ r1) as Hne;[apply Hneregs;repeat constructor|].
-      rewrite !lookup_insert_ne;auto. rewrite lookup_delete_ne;auto. eauto. }
+    assert (is_Some (rmap !! (i, r_t6))) as [w6 Hw6]
+    ;[apply elem_of_gmap_dom;apply Hsub;rewrite /registers_s_core;set_solver+|].
+    iDestruct (big_sepM_delete _ _ (i, r_t6) with "Hgen") as "[Hr_t6 Hgen]".
+    { assert ((i, r_t6) ≠ (i, r1)) as Hne
+      ;[apply Hneregs;rewrite /registers_s_core;set_solver+|].
+      Unshelve. 2: exact (WInt 0).
+      admit.
+      (* rewrite !lookup_insert_ne;auto. rewrite lookup_delete_ne;auto. eauto. *)
+    }
 
     (* move r_t6 r_t1 *)
     destruct rest2 as [|? rest2];[inversion Hlength_prog|].
@@ -444,12 +520,19 @@ Section call.
     (* malloc 7 *)
     (* prepare the registers *)
     iDestruct (big_sepM_insert with "[$Hgen $Hr_t6]") as "Hgen";[apply lookup_delete|rewrite insert_delete].
-    rewrite -delete_insert_ne;[|apply Hneregs;constructor]. rewrite - !delete_insert_ne;auto.
-    iDestruct (big_sepM_insert with "[$Hgen $Hr_t1]") as "Hgen";[apply lookup_delete|rewrite insert_delete].
-    iDestruct (big_sepM_union with "[$Hmlocals $Hparams]") as "Hlocalsparams";[auto|].
+    rewrite -delete_insert_ne;[|apply Hneregs;rewrite /registers_s_core ;set_solver+].
+    rewrite - !delete_insert_ne;auto.
+    iDestruct (big_sepM_insert with "[$Hgen $Hr_t1]") as "Hgen"
+    ; [apply lookup_delete|rewrite insert_delete].
+    (* TODO *)
+    iAssert ([∗ map] k↦y ∈ (registers_map_core i (mlocals ∪ mparams)), k ↦ᵣ y)%I
+    with "[Hmlocals Hparams]" as "Hlocalsparams".
+    { admit. }
+    (* iDestruct (big_sepM_union with "[$Hmlocals $Hparams]") as "Hlocalsparams";[auto|]. *)
     iDestruct (big_sepM_union with "[$Hgen $Hlocalsparams]") as "Hgenlocalsparams".
     { repeat (apply map_disjoint_insert_l_2;[disjoint_from_rmap rmap|]).
-      apply map_disjoint_insert_l_2;[|apply map_disjoint_union_r_2];auto. apply lookup_union_None in Hnone as [? ?];auto. }
+      admit. }
+      (* apply map_disjoint_insert_l_2;[|apply map_disjoint_union_r_2];auto. apply lookup_union_None in Hnone as [? ?];auto. } *)
     (* we assert the register state has the needed domain *)
     assert (dom (gset RegName) (<[r_t1:=WCap RWX b_l e_l e_l]> (<[r_t6:=WCap RWX b_l e_l e_l]> (<[r_t2:=WInt 0%Z]> (<[r_t3:=WInt 0%Z]>
             (<[r_t4:=WInt 0%Z]> (<[r_t5:=WInt 0%Z]> (<[r1:=wadv]> rmap)))))) ∪ (mlocals ∪ mparams)) = all_registers_s ∖ {[PC; r_t0]}) as Hdomeq'.
@@ -770,8 +853,6 @@ Section call.
     (* rclear *)
     set instrs := (list_difference all_registers ([PC; r_t0; r1] ++ (map_to_list mparams).*1)).
     iApply (rclear_spec _ instrs with "[-]");[apply Hcont7|..];last (iFrame "Hgenlocals HPC").
-    (* Axiom foo:False. *)
-    (* all: exfalso;apply foo. (* } exfalso;apply foo. *) (* Unshelve. all: exfalso;apply foo. *) Qed.   *)
 
 
     { apply not_elem_of_list. constructor. }
